QuickChick for add and multiplication circuits

VOQC/src/BooleanCompilation.v
@@ -29,7 +29,8 @@ Inductive bexp :=
 | b_f   : bexp
 | b_var : nat -> bexp
 | b_and : bexp -> bexp -> bexp 
-| b_xor : bexp -> bexp -> bexp.
+| b_xor : bexp -> bexp -> bexp
+| b_or : bexp -> bexp -> bexp.
 
 Fixpoint interpret_bexp (b : bexp) (f : nat -> bool) : bool :=
   match b with
@@ -38,6 +39,7 @@ Fixpoint interpret_bexp (b : bexp) (f : nat -> bool) : bool :=
   | b_var v     => f v 
   | b_and b1 b2 => (interpret_bexp b1 f) && (interpret_bexp b2 f)
   | b_xor b1 b2 => (interpret_bexp b1 f) ⊕ (interpret_bexp b2 f)
+  | b_or b1 b2 => (interpret_bexp b1 f) || (interpret_bexp b2 f)
   end.  
 
 Inductive bexp_well_typed : nat -> bexp -> Prop :=
@@ -45,7 +47,8 @@ Inductive bexp_well_typed : nat -> bexp -> Prop :=
   | WT_b_f : forall n, bexp_well_typed n b_f
   | WT_b_var : forall n q, (q < n)%nat -> bexp_well_typed n (b_var q)
   | WT_b_and : forall n b1 b2, bexp_well_typed n b1 -> bexp_well_typed n b2 -> bexp_well_typed n (b_and b1 b2)
-  | WT_b_xor : forall n b1 b2, bexp_well_typed n b1 -> bexp_well_typed n b2 -> bexp_well_typed n (b_xor b1 b2).
+  | WT_b_xor : forall n b1 b2, bexp_well_typed n b1 -> bexp_well_typed n b2 -> bexp_well_typed n (b_xor b1 b2)
+  | WT_b_or : forall n b1 b2, bexp_well_typed n b1 -> bexp_well_typed n b2 -> bexp_well_typed n (b_or b1 b2) .
 
 Lemma well_typed_increase_dim : forall b n n',
   (n <= n')%nat ->
@@ -73,6 +76,9 @@ Proof.
   - rewrite IHbexp_well_typed1; try assumption.
     rewrite IHbexp_well_typed2; try assumption.
     reflexivity.
+    - rewrite IHbexp_well_typed1; try assumption.
+    rewrite IHbexp_well_typed2; try assumption.
+    reflexivity.
 Qed.
 
 Lemma interpret_bexp_update : forall b f i j r,
@@ -95,6 +101,7 @@ Fixpoint max_var b v :=
   | b_var v' => max v v'
   | b_and b1 b2 => max (max_var b1 v) (max_var b2 v)
   | b_xor b1 b2 => max (max_var b1 v) (max_var b2 v)
+  | b_or b1 b2 => max (max_var b1 v) (max_var b2 v)
   | _ => v
   end.
 
@@ -103,6 +110,7 @@ Fixpoint no_vars b :=
   | b_var _ => false
   | b_and b1 b2 => no_vars b1 && no_vars b2
   | b_xor b1 b2 => no_vars b1 && no_vars b2
+  | b_or b1 b2 => no_vars b1 && no_vars b2
   | _ => true
   end.
 
@@ -130,13 +138,21 @@ Proof.
     + apply well_typed_increase_dim with (n:=num_inputs b2); try assumption.
       unfold num_inputs.
       simpl; destruct (no_vars b1); destruct (no_vars b2); simpl; lia.
+        - constructor.
+    + apply well_typed_increase_dim with (n:=num_inputs b1); try assumption.
+      unfold num_inputs.
+      simpl; destruct (no_vars b1); destruct (no_vars b2); simpl; lia.
+    + apply well_typed_increase_dim with (n:=num_inputs b2); try assumption.
+      unfold num_inputs.
+      simpl; destruct (no_vars b1); destruct (no_vars b2); simpl; lia.
 Qed.
 
 (* How many ancillary qubits are needed to represent this expression? *)
 Fixpoint num_ancillae b : nat :=
   match b with
   | b_and b1 b2 => 2 + (max (num_ancillae b1) (num_ancillae b2))
-  | b_xor b1 b2 => max (num_ancillae b1) (num_ancillae b2) 
+  | b_xor b1 b2 => max (num_ancillae b1) (num_ancillae b2)
+  | b_or b1 b2 => 2 + (max (num_ancillae b1) (num_ancillae b2))
   | _ => 0
   end.
 
@@ -148,6 +164,7 @@ Notation "p1 ; p2" := (bcseq p1 p2) (at level 50).
    program should only modify the qubit at index i.
    - i is the index of the result
    - j is the index of the next available ancilla. *)
+ 
 Fixpoint compile'  (b : bexp) (i j : nat) : bccom :=
   match b with
   | b_t         => bcx i
@@ -159,7 +176,14 @@ Fixpoint compile'  (b : bexp) (i j : nat) : bccom :=
                   compile' b2 (j+1) (j+2); 
                   compile' b1 j (j+2)
   | b_xor b1 b2 => compile' b1 i j; 
-                  compile' b2 i j
+                   compile' b2 i j
+  | b_or b1 b2 => compile' b1 j (j + 2);
+                  compile' b2 (j+1) (j + 2);
+                 bcccnot  j (j+1) i;
+                compile' b2 (j+1) (j +2 );
+                  compile' b1 j (j + 2);
+                  compile' b1 i (j + 2);
+                  compile' b2 i (j + 2)
   end.
 
 Definition compile b : bccom := 
@@ -181,7 +205,224 @@ Lemma cnot_false : forall (n i : nat) (f : nat -> bool),
 
 Local Opaque CCX.
 
+Lemma and_xor_xor : forall (b1 b2 : bool),
+    xorb (b1 && b2) (xorb b1 b2) = orb b1 b2.
+Proof.
+  intros.
+  destruct b1; 
+    destruct b2;
+    auto.
+Qed.   
 
+Lemma bcseq_assoc : forall (b1 b2 b3 : bccom) (f : nat -> bool),
+    bcexec(bcseq (bcseq b1 b2) b3) f = bcexec( bcseq b1 ( bcseq b2 b3)) f.
+  Proof. 
+    intros.
+    generalize dependent b2.
+    generalize dependent b3.
+    generalize dependent f. 
+    induction b1; intros; simpl; reflexivity. 
+    Qed. 
+(* 
+ bcexec
+    (compile' b1 j (j + 2);
+     (compile' b2 (j + 1) (j + 2);
+      (bcccnot j (j + 1) i; (compile' b2 (j + 1) (j + 2); compile' b1 j (j + 2))))) f =
+  f [i |-> f i ⊕ (interpret_bexp b1 f && interpret_bexp b2 f)]
+ *)
+
+  Lemma bcseq_update : forall (b1 b2 : bccom) (f : nat -> bool),
+      bcexec ( bcseq b1 b2 ) f = bcexec b2 (bcexec b1 f).
+  Proof.
+    intros.
+    generalize dependent b2.
+    generalize dependent f.
+    induction b1; simpl; reflexivity. 
+    Qed. 
+
+
+Lemma compile'_and_correct : forall dim (b1 b2 : bexp) (f : nat -> bool) (i j : nat),
+  bexp_well_typed i (b_and b1 b2) -> 
+  (i < j)%nat ->
+  (j + (num_ancillae (b_and b1 b2)) < dim + 1)%nat ->
+  (forall k, (k > i)%nat -> f k = false) ->
+  (forall i : nat,
+         bexp_well_typed i b1 ->
+         forall j : nat,
+         (i < j)%nat ->
+         (j + num_ancillae b1 < dim + 1)%nat ->
+         forall f : nat -> bool,
+         (forall k : nat, (k > i)%nat -> f k = false) ->
+         bcexec (compile' b1 i j) f = f [i |-> f i ⊕ interpret_bexp b1 f]) ->
+  (forall i : nat,
+         bexp_well_typed i b2 ->
+         forall j : nat,
+         (i < j)%nat ->
+         (j + num_ancillae b2 < dim + 1)%nat ->
+         forall f : nat -> bool,
+         (forall k : nat, (k > i)%nat -> f k = false) ->
+         bcexec (compile' b2 i j) f = f [i |-> f i ⊕ interpret_bexp b2 f]) ->
+  (bcexec (compile' b1 j (j+2); 
+                  compile' b2 (j+1) (j+2);
+                  bcccnot j (j+1) i;
+                  compile' b2 (j+1) (j+2); 
+                  compile' b1 j (j+2))) f
+    = (update f i ((f i) ⊕ (interpret_bexp (b_and b1 b2) f))).
+Proof.
+    intros dim b1 b2 f i j H H0 H1 H2 IHb1 IHb2.
+    inversion H; subst; clear H.
+    assert (bexp_well_typed j b1).
+    { apply (well_typed_increase_dim b1 i j); try assumption; lia. }
+    assert (bexp_well_typed (j+1) b2).
+    { apply (well_typed_increase_dim b2 i (j+1)); try assumption; lia. }
+    assert (j < j + 2)%nat by lia.
+    assert (j + 1 < j + 2)%nat by lia.
+    simpl in H1.
+    assert ((j + 2) + num_ancillae b1 < dim + 1)%nat by lia.
+    assert ((j + 2) + num_ancillae b2 < dim + 1)%nat by lia.
+    specialize (IHb1 j H (j+2)%nat H4 H8).
+    specialize (IHb2 (j+1)%nat H3 (j+2)%nat H5 H9).
+    clear H H3 H4 H5 H8 H9. (* difficult because it isn't multiplying *)
+    
+    simpl compile'.
+    simpl interpret_bexp.
+    (*repeat rewrite Mmult_assoc.*)
+    repeat rewrite bcseq_assoc.
+    rewrite bcseq_update; try lia. 
+    rewrite IHb1.
+    
+    rewrite bcseq_update.
+    rewrite IHb2; try lia.
+
+    rewrite update_index_neq; try lia.
+    
+    rewrite bcseq_update.         
+    rewrite bcccnot_correct; try lia.
+    rewrite update_index_eq; try lia.
+    rewrite update_twice_neq; try lia.
+  
+    rewrite bcseq_update.
+    rewrite IHb2.
+    repeat rewrite update_twice_eq; try lia.
+
+    rewrite <-  interpret_bexp_f with (i:= j) (f:=f) (f' := f [j |-> f j ⊕ interpret_bexp b1 f]).
+    repeat rewrite update_index_eq.
+    rewrite update_index_neq; try lia.
+
+    rewrite IHb1.
+    rewrite update_index_neq; try lia.
+    rewrite update_index_neq; try lia.
+    rewrite update_twice_neq; try lia.
+    rewrite update_index_eq; try lia.
+    rewrite update_index_neq; try lia.
+    rewrite update_index_neq; try lia.
+    assert ((f (j + 1) %nat) = false).
+    apply H2; try lia.
+    assert ((f (j) %nat) = false).
+    apply H2; try lia.
+    rewrite H.
+    rewrite H3.
+
+    rewrite xorb_false_l.
+    rewrite xorb_false_l.
+    rewrite update_index_eq.
+    
+    rewrite (update_twice_neq _ (j)); try lia.
+    rewrite (update_twice_neq _ (j)); try lia.
+    rewrite <-  interpret_bexp_f with (i:= i) (f:=f)
+             (f' := (((f [i |-> f i ⊕ (interpret_bexp b2 f && interpret_bexp b1 f)]) [j
+             |-> interpret_bexp b1 f]) [j + 1 |-> interpret_bexp b2 f])).
+    rewrite <-  interpret_bexp_f with (i:= i) (f:=f)
+             (f' := (((f [i |-> f i ⊕ (interpret_bexp b2 f && interpret_bexp b1 f)]) [j
+            |-> interpret_bexp b1 f]) [j + 1 |-> interpret_bexp b2 f ⊕ interpret_bexp b2 f])).
+    rewrite xorb_nilpotent.
+    rewrite xorb_nilpotent.
+    rewrite update_twice_neq; try lia.
+    rewrite update_twice_eq; try lia.
+    rewrite update_same; try lia.
+    rewrite update_same; try lia.
+    rewrite andb_comm.    
+    reflexivity.
+
+    rewrite update_index_neq; try lia.
+    rewrite H3.
+    reflexivity.
+
+    rewrite update_index_neq; try lia.
+    rewrite update_index_neq; try lia.
+    rewrite H2; try lia.
+    reflexivity.
+
+    apply H6.
+
+    intros; repeat (rewrite update_index_neq; try lia); try reflexivity.
+
+    apply H7.
+
+    intros; repeat (rewrite update_index_neq; try lia); try reflexivity.
+
+    intros.
+    rewrite update_twice_neq; try lia.
+    rewrite update_index_neq; try lia.
+    rewrite update_twice_neq; try lia.
+    rewrite update_index_neq; try lia.
+    assert ((f (j + 1) %nat) = false).
+    apply H2; try lia.
+    assert ((f (j) %nat) = false).
+    apply H2; try lia.
+    rewrite H3.
+    rewrite H4.
+    rewrite xorb_false_l.
+    rewrite xorb_false_l.
+    rewrite <-  interpret_bexp_f with (i:= i) (f:=f)
+             (f' := (((f [j |-> interpret_bexp b1 f]) [i
+             |-> (f [j |-> interpret_bexp b1 f]) i
+                 ⊕ (interpret_bexp b2 f &&
+                    ((f [j |-> interpret_bexp b1 f]) [j + 1 |-> interpret_bexp b2 f]) j)]) [
+            j + 1 |-> interpret_bexp b2 f])); try lia.
+    rewrite xorb_nilpotent.
+    rewrite update_same.
+    apply H2; lia.
+    symmetry. apply H3.
+
+    apply H7.
+
+    intros.
+    rewrite update_index_neq; try lia.
+    rewrite update_index_neq; try lia.
+    rewrite update_index_neq; try lia.
+    reflexivity.
+
+    apply well_typed_increase_dim with (n:=i)(n':=j); try lia. apply H7.
+
+    intros.
+    rewrite update_index_neq; try lia; reflexivity.
+
+    intros.
+    rewrite update_twice_neq; try lia.
+    rewrite update_index_neq; try lia.
+    rewrite update_twice_neq; try lia.
+    rewrite update_index_neq; try lia.
+    assert ((f (j + 1) %nat) = false).
+    apply H2; try lia.
+    assert ((f (j) %nat) = false).
+    apply H2; try lia.
+    rewrite H3.
+    rewrite H4.
+    rewrite xorb_false_l.
+    rewrite xorb_false_l.
+    rewrite update_index_neq; try lia.
+    apply H2; try lia.
+
+    intros.
+    rewrite update_index_neq; try lia.
+    apply H2; try lia.
+
+    intros.
+    apply H2; try lia.
+Qed.    (* END AND *)
+
+  
 Lemma compile'_correct : forall dim (b : bexp) (f : nat -> bool) (i j : nat),
   bexp_well_typed i b -> 
   (i < j)%nat ->
@@ -213,80 +454,18 @@ Proof.
     + reflexivity.
     + rewrite xorb_false_r.
       rewrite update_same;
-      reflexivity. 
-      - (* b_and b1 b2 *) 
-    inversion H; subst; clear H.
-    assert (bexp_well_typed j b1).
-    { apply (well_typed_increase_dim b1 i j); try assumption; lia. }
-    assert (bexp_well_typed (j+1) b2).
-    { apply (well_typed_increase_dim b2 i (j+1)); try assumption; lia. }
-    assert (j < j + 2)%nat by lia.
-    assert (j + 1 < j + 2)%nat by lia.
-    simpl in H1.
-    assert ((j + 2) + num_ancillae b1 < dim + 1)%nat by lia.
-    assert ((j + 2) + num_ancillae b2 < dim + 1)%nat by lia.
-    specialize (IHb1 j H (j+2)%nat H4 H8).
-    specialize (IHb2 (j+1)%nat H3 (j+2)%nat H5 H9).
-    clear H H3 H4 H5 H8 H9. (* difficult because it isn't multiplying *)
-    
-    simpl.
-    (*repeat rewrite Mmult_assoc.*)
-    rewrite IHb1.
-    2: { intros.
-         BreakIf.
-         BreakIf.
-         rewrite update_same.
-                  
-          
-         
+        reflexivity.
 
-         apply H2. lia. }
-    rewrite IHb2.
-    2: { intros. rewrite update_index_neq; try apply H2; lia. }
-    rewrite update_index_neq; try lia.
-    rewrite <- interpret_bexp_update with (i:=i);
-      try assumption; try lia.
-    rewrite f_to_vec_CCX; try lia.
-    rewrite update_index_eq. 
-    do 3 (rewrite update_index_neq; try lia).
-    rewrite update_index_eq.
-    rewrite IHb2.
-    2: { intros. repeat rewrite update_index_neq; try apply H2; lia. }
-    rewrite (update_twice_neq _ (j+1)); try lia.
-    rewrite update_twice_eq. 
-    rewrite update_index_eq.
-    repeat rewrite <- interpret_bexp_update with (i:=i);
-      try assumption; try lia.
-    rewrite xorb_assoc.
-    rewrite xorb_nilpotent.
-    rewrite xorb_false_r.
-    rewrite IHb1.
-    2: { intros. 
-         rewrite update_twice_neq; try lia.
-         rewrite update_index_neq; try lia.
-         rewrite update_twice_neq; try lia.
-         rewrite update_index_neq; try lia.
-         rewrite update_same; try reflexivity.
-         apply H2; lia. }
-    do 2 (rewrite (update_twice_neq _ j); try lia).
-    rewrite update_twice_eq.
-    rewrite update_index_eq.
-    repeat rewrite <- interpret_bexp_update with (i:=i);
-      try assumption; try lia.
-    rewrite xorb_assoc.
-    rewrite xorb_nilpotent.
-    rewrite xorb_false_r.
-    repeat rewrite (update_twice_neq _ i); try lia.
-    rewrite (update_same _ (j+1)); try reflexivity.
-    rewrite (update_same _ j); try reflexivity.
-    rewrite H2 with (k:=j); try lia.
-    rewrite H2 with (k:=(j+1)%nat); try lia.
-    repeat rewrite xorb_false_l.
-    reflexivity.
+      
+  - (* b_and b1 b2 *)
+    simpl compile'.
+    apply compile'_and_correct with (dim:= dim); auto.
+
   - (* b_xor b1 b2 *)
     inversion H; subst; clear H.
     simpl.
-    rewrite Mmult_assoc.
+
+    
     simpl in H1.
     rewrite IHb1; try assumption; try lia.
     rewrite IHb2; try assumption; try lia.
@@ -297,13 +476,57 @@ Proof.
       try assumption; try lia.
     rewrite xorb_assoc.
     reflexivity.
-Qed.
 
+  -
+    simpl compile'.
+    rewrite bcseq_assoc.
+    rewrite bcseq_update.
+    
+    inversion H; subst; clear H.
+    assert (bexp_well_typed j b1).
+    { apply (well_typed_increase_dim b1 i j); try assumption; lia. }
+    assert (bexp_well_typed (j+1) b2).
+    { apply (well_typed_increase_dim b2 i (j+1)); try assumption; lia. }
+    assert (j < j + 2)%nat by lia.
+    assert (j + 1 < j + 2)%nat by lia.
+    simpl in H1.
+    assert ((j + 2) + num_ancillae b1 < dim + 1)%nat by lia.
+    assert ((j + 2) + num_ancillae b2 < dim + 1)%nat by lia.
+    clear H H3 H4 H5 H8 H9. (* difficult because it isn't multiplying *)
+
+    
+    rewrite compile'_and_correct with (dim:= dim); auto; try constructor; try assumption.
+    rewrite bcseq_update.
+    rewrite IHb1;  auto;  try lia.
+    rewrite update_index_eq.
+    rewrite update_twice_eq.
+    simpl interpret_bexp.
+    rewrite <- interpret_bexp_update with (i:=i); try assumption; try lia.
+    
+        
+    rewrite IHb2;  auto;  try lia.
+    rewrite update_index_eq.
+    rewrite update_twice_eq.
+    rewrite <- interpret_bexp_update with (i:=i); try assumption; try lia.
+
+    rewrite xorb_assoc.
+    rewrite xorb_assoc.
+    rewrite and_xor_xor.
+    reflexivity.
+
+    intros.
+    rewrite update_index_neq; auto; try lia.
+
+    intros.
+    rewrite update_index_neq; auto; try lia.
+Qed.
+(*
 Lemma compile_correct : forall (b : bexp) (f : nat -> bool) (r : bool), 
   let in_s := fun i => if i <? (num_inputs b) then f i else false in
   let out_s := update in_s (num_inputs b) (interpret_bexp b f) in
   (@uc_eval (b_dim b) (compile b)) × f_to_vec (b_dim b) in_s
-    = f_to_vec (b_dim b) out_s.
+  = f_to_vec (b_dim b) out_s.
+ 
 Proof.
   intros.
   unfold compile, out_s.
@@ -319,7 +542,7 @@ Proof.
     try (contradict H; lia); reflexivity.
   intros k Hk. unfold in_s. bdestruct (k <? num_inputs b);
     try (contradict H; lia); reflexivity.
-Qed.
+Qed.*)
 
 (** Examples **)
 (* Small examples taken from (Re)QWIRE's Arithmetic.v file.
