VOQC/src/numbers.v
@@ -1,0 +1,736 @@
+Require Import UnitaryOps.
+Require Import BooleanCompilation.
+Require Import Coq.NArith.NArith.
+Require Import BinNums.
+Require Import RCIR.
+From QuickChick Require Import QuickChick. Import QcNotation.
+
+(* Suppress some annoying warnings: *)
+Set Warnings "-extraction-opaque-accessed,-extraction".
+
+Require Export ExtLib.Structures.Monads.
+Export MonadNotation. Open Scope monad_scope.
+
+Require Import String.  Local Open Scope string.
+
+(*********************************)
+(** Natural Number Compilation **)
+(*********************************)
+(* This file defines a 'compile' function that converts an arbitrary
+   numeric expression into a reversible circuit that (provably) uncomputes 
+   its ancillae. We use eager ancilla cleanup, which requires fewer qubits,
+   but more gates, than the lazy approach. Because SQIR does not allow
+   initializing / discarding qubits, we precompute the number of ancillae
+   needed and include them in the global register.
+ 
+   The numeric expression language and compilation strategy are modelled
+   after the BooleanCompilation.v file, also found in VOQC, which is 
+   itself based on the ReVerC reversible circuit compiler.
+   In particular, this compilation process uses boolean circuits constructed
+   from BooleanCompilation in order to streamline the circuit creation process.
+
+
+   We prove that compilation is correct by showing that the output circuit
+   has the expected behavior on any basis state. The proof requires some
+   new formalisms for describing classical states (see 'f_to_vec'). *)
+
+(** Natural Number Expressions **)
+
+(*The general strategy to represent natural numbers is by logically 
+  partitioning our bits into fixed sized registers. This size is defined
+  when calling the compile function, and is passed into nearly every function. 
+   *)
+
+(*Throughout this file, Coq nats can have three different meanings:
+1) nat representing a register. An example of this is the argument of 
+  n_var_reg, in which a nat is used to select a register. For instance,
+  n_var_reg 1 represents bits reg_size through 2*reg_size -1, where reg_size
+  is the defined register size
+
+2) nat representing a register-sized group of bits beginning with the
+   argument-th bit. An example of this would be 
+   n_var_bit 1, which would represent bits 1 through reg_size, where
+   reg_size is the defined register size. 
+   
+This use of nats is prevalently used throughout the compilation process
+   via parameters i and j, with i typically representing the first bit of 
+   a register or a target bit and j representing the first usable ancilla bit
+
+3) An actual number, typically representing either the size of a register 
+   (or some variable which tracks the size of a number throughout a recursive
+   function) or the actual value of a nexp itself, such as the output of interpret_nexp
+
+ *)
+(*As an example, here is a representation of the number 3 and 4 loaded into
+  the first two registers of size 4, with 20 total bits:
+  0011 0100 0000 0000 0000 
+
+  The compilation with place a result into the first unused register, in this case most likely the third register. 
+
+  Compiling n_var_reg 0 will leave us with bits:
+  0011 0100 0011 0000 0000
+  as it copies over the first register
+
+  Compiling n_var_bit 2 will leave us with bits:
+  0011 0100 1101 0000 0000
+  as it copies over bits 2 through 5
+
+  Compiling n_plus (n_var_reg 0) (n_var_reg 1) gives us:
+  0011 0100 0111 0000 0000
+  with 0111 = 7 being the sum of 3 and 4. Note that this would need more ancilla 
+  than is shown.
+
+  Compiling n_mult (n_var_reg 0) (n_var_reg 1) gives us:
+  0011 0100 1100 0000 0000
+  with 0111 = 12 being the product of 3 and 4. Note that this would need more ancilla 
+  than is shown.
+
+*)
+Inductive  nexp :=
+| n_var_reg : nat -> nexp (*register number 0-indexed nat -> nexp *)
+| n_var_bit : nat -> nexp (*uses an arbitrary register's worth of bits beginning at nat -> nexp*)
+| n_plus : nexp -> nexp -> nexp
+| n_shiftr : nexp -> nat -> nexp 
+| n_mult : nexp -> nexp -> nexp.
+
+(*shift_vec_l is used in order to isolate the natural number value represented by a group of bits.
+interpret_nexp shifts a group of bits to the left so that the first bit of the group is seen as 
+(f 0). This is needed because funbool_to_nat (which is defined in VectorStates.v in SQIR) works
+by converting our function to a list, and then calculating a natural number from the first
+*size* values of that list. shift_l allows us to push our desired group of numbers to the first 
+value in the list and allows funbool_to_nat to ignore any prior bits *)
+Definition shift_vec_l {A} (input_vec : nat -> A) k := fun i => input_vec (i + k)%nat.
+(*make lemmas for this *)   
+
+(*calculates the value of nexps. Uses funbool_to_nat as explained above shift_l.
+  the f defines the space of bit values that we want to interpret.  *)
+Fixpoint interpret_nexp (n : nexp) (input_vec : nat -> bool) (register_size : nat): nat :=
+  match n with
+  | n_var_reg e1 => funbool_to_nat register_size (shift_vec_l input_vec (e1 * register_size))
+  | n_var_bit e1 => funbool_to_nat register_size (shift_vec_l input_vec (e1))                 
+  | n_plus e1 e2 => (interpret_nexp e1 input_vec register_size)
+                    + (interpret_nexp e2 input_vec register_size)
+  | n_shiftr e1 c => (interpret_nexp e1 input_vec register_size)
+                     * (2 ^ c)
+  | n_mult e1 e2 => (interpret_nexp e1 input_vec register_size)
+                    * (interpret_nexp e2 input_vec register_size)
+  end. 
+
+(*
+Example of interpret_nexp: 
+
+practicef builds a space of bits with bits 0 and 1 being activated
+  interpret_nexp knows that (n_var_ reg 0) represents bits 0 through 3
+  because the value 4 is being passed in as register_size. 
+
+interpret_nexp then shifts practicef by 0, because we access the 0th register.
+
+Then, funbool_to_nat turns our f (defined below and unmodified by shift_l) 
+into the list [false, false, true, true], again, because the register_size is 4. From this list
+is calculated the value 3, which has a binary representation corresponding to the list
+where false = 1 and true = 0.
+
+We could define any arbitrary f to input into interpret_nexp,
+and that would change the output. 
+    
+ *)
+Definition practiceInput : nat -> bool :=
+  fun n => (match n with
+            |0 => false
+            |S 0 => true
+            |_ => true end).
+
+Eval compute in interpret_nexp (n_var_reg 0)  practiceInput 4.
+
+Definition f_in : nat -> bool :=
+  fun n => (match n with
+            |0 => false
+            |S 0  => false
+            |S (S 0) => false
+            |S (S (S 0)) => true
+
+                    
+            |4 => false
+            |5 => false
+            |6 => true
+            |7 => true
+            |_ => true end).
+Eval compute in funbool_to_list 4 (shift_vec_l f_in 1).
+Eval compute in interpret_nexp (n_var_reg 0) f_in 4.
+Eval compute in interpret_nexp (n_var_reg 1) f_in 4.
+
+(*Only reversible if number is well typed for shiftr, but this is up to the user to define
+a large enough register size. Could (possibly) include this in well_typed? *)                     (*A nexp is well typed if the bits it is trying to access are within the total number of input bits *)                                                          
+Inductive nexp_well_typed (register_size : nat) : nat -> nexp -> Prop :=
+| WT_n_var_reg : forall n q, (q * register_size < n)%nat -> nexp_well_typed register_size n (n_var_reg q )
+                                                            
+| WT_n_var_bit : forall n q, (q < n)%nat -> nexp_well_typed register_size n (n_var_bit q )
+| WT_n_plus : forall n n1 n2, nexp_well_typed register_size n n1 ->
+                              nexp_well_typed register_size n n2 ->
+                              nexp_well_typed register_size n (n_plus n1 n2)
+| WT_n_shiftr : forall n n1 s, nexp_well_typed register_size n n1 ->
+                               nexp_well_typed register_size n (n_shiftr n1 s)
+| WT_n_mult : forall n n1 n2, nexp_well_typed register_size n n1 ->
+                              nexp_well_typed register_size n n2 ->
+                              nexp_well_typed register_size n (n_mult n1 n2).
+
+(*Have not fully worked out n_well_typed_increase_dim and
+interpret_nexp_f yet *)
+Lemma n_well_typed_increase_dim : forall e n n' size,
+    (n <= n')%nat ->
+    nexp_well_typed size n e ->
+    nexp_well_typed size n' e.
+Proof.
+  intros.
+  induction H0; try constructor; try lia; try auto.
+Qed.
+    
+(*TODO. Unsure as to how I want to express these lemmas, whether with registers or bits *)
+Lemma interpret_nexp_f : forall i n f f' size,
+    nexp_well_typed size i n ->
+    (forall k, (k < i)%nat -> f k = f' k) ->
+    interpret_nexp n f = interpret_nexp n f'.
+Proof.
+  intros.
+  induction H; simpl; try reflexivity.
+  
+ Admitted. (*
+  intros.
+  induction H; simpl; try reflexivity.
+  - unfold shift_l. apply H0. (* FIX THIS*)
+  rewrite IHnexp_well_typed1.
+  rewrite IHnexp_well_typed2.
+  reflexivity.
+  apply H0.
+  apply H0.*)
+
+
+
+(** Compilation of boolean expressions to oracles **)
+
+(* How many input variables does this expression use? *)
+
+(*n_max_var calculates the number of inputs used by  our nexp.
+  Conveniently, it will return a number which corresponds with
+  the first bit of the register that will store our result.
+
+  Perhaps could be renamed a bit more clearly. 
+  
+  This should align with every other register unless you use n_var_bit
+ *)
+
+
+Fixpoint n_num_input_bits (n : nexp) ( register_size: nat) :=
+  match n with
+  | n_var_reg n1 => (register_size * (n1 + 1))%nat
+  | n_var_bit n1 => (n1 + register_size)%nat
+  | n_plus n1 n2 =>  ((max (n_num_input_bits n1 register_size)
+                           (n_num_input_bits n2 register_size)))%nat
+  | n_shiftr n1 s => n_num_input_bits n1  register_size
+  | n_mult n1 n2 => ((max (n_num_input_bits n1 register_size)
+                          (n_num_input_bits n2 register_size)))%nat
+  end.
+
+(*n_plus will add the number stored by bits 0-3 and the number stored by bits 4-7. 
+  n_num_input_bits (n_var_reg 0) returns 4 (because 0 through 3 are clearly occupied)
+  n_num_input_bits (n_var_reg 1) returns 8 (because 4 through 7 are clearly occupied)
+  Therefore the overrall n_num_input_bits returns 8. Meaning that we can store our output
+  beginning with bit 8. *)
+Eval compute in n_num_input_bits (n_plus (n_var_reg 0) (n_var_reg 1)) 4.
+
+(*Lemma n_num_inputs_well_typed : forall n,
+    nexp_well_typed (n_num_inputs n) n.
+Proof.
+  induction n.
+  - constructor. unfold n_num_inputs; simpl. lia.  
+  - constructor.
+    + apply n_well_typed_increase_dim with (n:=n_num_inputs n1); try assumption.
+      unfold n_num_inputs. simpl. lia.
+    + apply n_well_typed_increase_dim with (n:= n_num_inputs n2); try assumption.
+      unfold n_num_inputs. simpl. lia.
+Qed.
+*)
+
+(*This most likely isn't needed anymore unless we decide not to use 
+fixed sized registers *)
+Fixpoint n_num_out n (register_size : nat): nat :=
+  match n with
+  | n_var_reg n1  => register_size
+  | n_var_bit n1 => register_size
+  | n_plus n1 n2 => register_size
+  | n_shiftr n1 s => register_size
+  | n_mult n1 n2 => register_size
+  end.
+
+(*These are very much incorrect but not used, will fix. This will be used to 
+calculate the total number of ancilla for each circuit, which will allow us to 
+precompute the total number of bits we'll used (shown by n_dim)*)
+
+Fixpoint n_num_ancillae n (register_size : nat) : nat :=
+  match n with
+  | n_plus n1 n2 => register_size * 3 +2 (*Three registers (n1, n2, carries) plus 2 ancillae *)
+  | n_mult n1 n2 => register_size *(3 + register_size)+ (register_size * 3) + 2 (*TODO *)
+  | _ => 0
+  end.
+  
+(* Total number of qubits required. *)
+Definition n_dim (n : nexp) (register_size : nat) : nat :=
+  (n_num_input_bits n register_size) +
+  (n_num_out n register_size) +
+  (n_num_ancillae n register_size).
+
+
+
+
+
+(*ripple carry adder*)
+Definition adder_cout_bexp (n1_bit n2_bit carry : nat) : bexp:= (b_var carry ∧ (b_var n2_bit ⊻ b_var n1_bit)) ⊻ (b_var n2_bit ∧ b_var n1_bit).
+Definition adder_sum_bexp (n1_bit n2_bit carry : nat) : bexp := (b_var carry) ⊻ (b_var n2_bit ⊻ b_var n1_bit).
+(*I will store carries in /the first/ register after the register I want to store my number in. Any other misc ancilla will be after the end of my carry register *)
+
+(* 
+|n0
+|n1
+|n2
+...
+|n
+
+|n1+n2 <- i_out
+|all the carries (eventually removed)
+|copy of n1 (eventually removed) <- i_in1
+|copy of n2 (eventually removed) <- i_in2
+| <- i_anc
+ *)
+(*recursive compilation for adding two numbers. 
+
+i_in1: bit we want to add of n1
+i_in2: bit we want to add of n2
+i_out: bit we want to store the sum in
+i_anc: first ancilla bit accessible (ancilla bit layout is shown above)
+n: decreasing nat showing how many bits are left to sum
+sz_reg: register size *)
+(*Renaming compile' to compile_bit for ease of readability *)
+Definition compile_bit  (e : bexp) (i_out i_anc : nat) : bccom :=
+  compile' e i_out i_anc.
+
+
+(*i_in1 and i_in2 begin as rightmost bit of numbers then move left *)
+Fixpoint n_compile_plus   (i_in1 i_in2 i_out i_anc n sz_reg: nat) : bccom:=
+  (* *)
+  match n with
+  | 0 => bcskip
+  (*Last bit means we don't need to store the carry *)
+  | S 0 =>     compile_bit (adder_sum_bexp i_in1 i_in2 (i_out + sz_reg)%nat) i_out i_anc
+  | S n' => 
+    compile_bit (adder_cout_bexp i_in1 i_in2 (i_out + sz_reg)%nat) (i_out + sz_reg - 1) i_anc;
+    compile_bit (adder_sum_bexp i_in1 i_in2 (i_out + sz_reg)%nat) i_out i_anc;
+    n_compile_plus (i_in1 - 1) (i_in2 - 1) (i_out - 1) i_anc (n') sz_reg;
+    compile_bit (adder_cout_bexp i_in1 i_in2 (i_out + sz_reg)%nat) (i_out + sz_reg - 1) i_anc
+end.
+
+(*n_compile_var is based off of BooleanCompilation.v's compilation of b_var.
+
+It copies each bit of the desired register into the output register
+ *)
+Fixpoint n_compile_var   (i_in i_out i_anc n sz_reg: nat) : bccom :=
+
+  match n with
+  |S n' => compile_bit (b_var i_in) i_out i_anc;
+              n_compile_var (i_in + 1) (i_out + 1) i_anc n' sz_reg
+  |0 => bcskip
+end.
+
+
+        
+(*n_compile_mult will multiply two numbers (hopefully)
+I want to do this using the logic of decomposing numbers into powers of 2.
+As an example, 6 = 2^2 + 2^1. My vision is for this to happen. 
+
+This copies each number to the next free register and shifts it
+it then adds this number to the last partial sum, and continues
+ *)
+
+(*n_compile_shiftl swaps each bit of a number with the bit to its left.
+  This is only reversible if we assume that the number is not too big for the register.
+
+  It performs the shift once *)
+Fixpoint n_compile_shiftl   ( i_curr i_anc n sz_reg : nat) : bccom :=
+  match n with
+  |0 => bcskip
+  |S 0 =>bcskip
+  |S n' => n_compile_shiftl (i_curr - 1) i_anc n' sz_reg;
+           bccnot i_curr (i_curr - 1); bccnot (i_curr - 1) i_curr
+            
+end.
+
+ (*n_compile_shiftr_c (c is for constant) does n_compile_shiftr multiple times *)
+Fixpoint n_compile_shiftl_c   (i_in i_anc c n sz_reg : nat) : bccom :=
+  match c with
+  |0 => bcskip
+  |S c' => n_compile_shiftl i_in i_anc n sz_reg;
+           n_compile_shiftl_c i_in i_anc c' n sz_reg
+end.
+(* Like shiftr but the opposite *)
+Fixpoint n_compile_shiftr   ( i_curr i_anc n sz_reg : nat) : bccom :=
+  match n with
+  |0 => bcskip
+  |S 0 =>bcskip
+  |S n' => bccnot (i_curr - 1) (i_curr) ; bccnot i_curr (i_curr - 1);
+                n_compile_shiftr (i_curr - 1) i_anc n' sz_reg
+               
+            
+end.
+
+ (*n_compile_shiftr_c (c is for constant) does n_compile_shiftr multiple times *)
+Fixpoint n_compile_shiftr_c   (i_in i_anc c n sz_reg : nat) : bccom :=
+  match c with
+  |0 => bcskip
+  |S c' => n_compile_shiftr i_in i_anc n sz_reg;
+           n_compile_shiftr_c i_in i_anc c' n sz_reg
+end.
+
+
+
+
+Fixpoint n_compile_and_bit_reg   (i_in i_if i_out i_anc n sz_reg : nat ) : bccom :=
+  match n with
+  | 0=> bcskip
+  | S n' => (compile_bit (b_and i_in i_if) i_out i_anc);
+            n_compile_and_bit_reg (i_in-1) i_if (i_out - 1) i_anc n' sz_reg
+  end.
+
+Definition n_compile_ifb_shift   (i_in i_if i_out i_anc  c sz_reg: nat) : bccom :=
+ 
+  n_compile_and_bit_reg i_in i_if i_out i_anc sz_reg sz_reg;
+  n_compile_shiftl_c i_out i_anc c sz_reg sz_reg.
+Definition n_compile_ifb_shift_rev   (i_in i_if i_out i_anc  c sz_reg: nat) : bccom :=
+
+  n_compile_shiftr_c i_out i_anc c sz_reg sz_reg;
+  n_compile_and_bit_reg i_in i_if i_out i_anc sz_reg sz_reg.
+ 
+      
+(*i_anc is first bit things should be copied to  *)
+(*i_in1 and i_in2 are the rightmost bit of their numbers, i_anc is leftmost free bit which is why I do the i_anc ... + sz_reg - 1. This goes to the rightmost bit of that register 
+
+a * b
+
+a ? + a>>1 + a>>2?
+0011 = 3
+0110 = 6
+1100 = 12
+
+0011 * 0111
+
+*)
+Fixpoint n_compile_mult   (i_in1 i_in2 i_out i_anc n c sz_reg: nat) : bccom :=
+  match n with
+  | 0 => n_compile_var (i_anc + sz_reg * (c + 1)) i_out i_anc sz_reg sz_reg
+  | S n' =>
+    n_compile_ifb_shift i_in1 i_in2 (i_anc + sz_reg - 1)
+                        (i_anc + sz_reg * sz_reg * 2) c sz_reg;
+
+    n_compile_plus (i_anc +sz_reg - 1) (i_anc + sz_reg * (c+2) - 1)
+               (i_anc + sz_reg * (c+3) - 1) (i_anc + sz_reg * sz_reg *2) sz_reg sz_reg; 
+
+    n_compile_ifb_shift_rev i_in1 i_in2 (i_anc + sz_reg - 1)
+                        (i_anc + sz_reg * sz_reg * 2) c sz_reg;
+
+    n_compile_mult i_in1 (i_in2 - 1) i_out (i_anc) n' (c + 1) sz_reg    
+end.
+
+Fixpoint n_compile_mult_cleanup   (i_in1 i_in2 i_out i_anc n c sz_reg: nat) : bccom :=
+  match n with
+  | 0 => bcskip
+           
+  | S n' =>
+            n_compile_ifb_shift i_in1 i_in2 (i_anc + sz_reg - 1)
+                        (i_anc + sz_reg * sz_reg * 2) (c -1) sz_reg;
+
+            n_compile_plus (i_anc +sz_reg - 1) (i_anc + sz_reg * (c+1) - 1)
+               (i_anc + sz_reg * (c+2) - 1) (i_anc + sz_reg * sz_reg *2) sz_reg sz_reg;
+
+            n_compile_ifb_shift_rev i_in1 i_in2 (i_anc + sz_reg - 1)
+                        (i_anc + sz_reg * sz_reg * 2) (c - 1) sz_reg;
+
+            n_compile_mult_cleanup i_in1 (i_in2 + 1) i_out (i_anc) n' (c - 1) sz_reg
+                    
+end.
+
+Fixpoint n_compile'   (e : nexp) (i_out i_anc sz_reg: nat) : bccom :=
+  match e with 
+  | n_var_reg e1 => n_compile_var (e1 * sz_reg) i_out i_anc sz_reg sz_reg 
+
+  | n_var_bit e1 => n_compile_var e1 i_out i_anc sz_reg sz_reg
+
+  | n_plus e1 e2 => n_compile' e1 (i_anc + sz_reg) (i_anc + sz_reg *2) sz_reg;
+                    n_compile' e2 (i_anc + sz_reg * 2) (i_anc + sz_reg *3) sz_reg;
+                    n_compile_plus (i_anc + sz_reg * 2 -1) (i_anc + sz_reg * 3 - 1)
+                                   (i_out + sz_reg - 1) (i_anc + sz_reg *3) sz_reg sz_reg;
+                    n_compile' e2 (i_anc + sz_reg *2) (i_anc + sz_reg *3) sz_reg;
+                    n_compile' e1 (i_anc + sz_reg) (i_anc + sz_reg *2) sz_reg
+
+  | n_shiftr e1 c => n_compile' e1 i_out i_anc sz_reg;
+                     n_compile_shiftr_c i_out i_anc c sz_reg sz_reg
+
+      | n_mult e1 e2 =>  n_compile' e1 (i_anc) (i_anc + sz_reg) sz_reg;
+                     
+                     n_compile' e2 (i_anc  + sz_reg) (i_anc + sz_reg *2) sz_reg;
+                     
+                     n_compile_mult (i_anc + sz_reg - 1) (i_anc + sz_reg + sz_reg - 1)
+                                     i_out (i_anc + sz_reg *2) sz_reg 0 sz_reg ;
+                     
+                     n_compile_mult_cleanup (i_anc + sz_reg - 1) (i_anc + sz_reg)
+                                     i_out (i_anc + sz_reg *2) sz_reg sz_reg sz_reg ; 
+                     
+                     n_compile' e2 (i_anc  + sz_reg) (i_anc + sz_reg *2) sz_reg;
+                     n_compile' e1 (i_anc) (i_anc + sz_reg) sz_reg
+
+
+  end. 
+
+(*compiles our number *)  
+Definition n_compile n r_size : bccom :=
+  n_compile' n (n_num_input_bits n r_size) ((n_num_input_bits n r_size) + r_size) r_size. 
+(* Correctness of compile':
+   1. The value at index i is xor-ed with the desired boolean expression.
+   2. All other values remain unchanged.
+
+   Notes:
+   * The well-typedness constraint is used in the b_var case.
+   * 'i < j' is used when applying f_to_vec_X, f_to_vec_bccnot, and f_to_vec_TOFF.
+   * 'j + (num_ancillae b) < n + 1' and 'forall k ...' are used in the b_and 
+     case -- note that this is the only case where the ancilla matter.
+*)
+Local Opaque CCX.
+
+     
+     (*
+Lemma n_compile'_correct : forall (n : nexp) (f : nat -> bool) (dim i j d: nat), (* d for digit (even though it's bits *)
+    nexp_well_typed i n -> (i < j)%nat -> (d < size n)%nat -> (j + (n_num_ancillae n) < dim + 1)%nat ->
+    (forall k, (k > i)%nat -> f k = false) ->  
+    (uc_eval (@n_compile' dim n i j 0)) × (f_to_vec dim f) =
+    f_to_vec dim (update f (i- d)%nat ((f (i - d)%nat) ⊕ (interpret_nexp_at n f d))).
+Proof.
+  intros.
+  generalize dependent f.
+  generalize dependent j.
+  generalize dependent i.
+  induction n; intros. (* Inductive structure of nexp *)
+  - inversion H; subst; clear H.
+    unfold n_compile'. unfold n_compile_val.
+    (* Induction on d *)
+   (* induction d.
+    + unfold interpret_nexp_at.
+      assert (n/(2 ^ 0) = n)%nat. simpl. apply Nat.div_1_r. rewrite H.
+      induction n0. unfold size. simpl in H1. autorewrite with eval_db. try lia. try lia.
+      destruct (n mod 2 =? 1).
+      2:{induction n. assert ((0 / 2) = 0 )%nat. apply Nat.div_small. lia. rewrite H4. rewrite IHn0. reflexivity. unfold size.  unfold size in H1. rewrite H1. }*)
+(*Induction on n0?*)
+    induction n. (* induction on value of the number *)
+    + unfold interpret_nexp_at. unfold size. simpl in H1.
+      rewrite Nat.div_0_l. rewrite Nat.mod_0_l.
+      induction n0. (*induction on number of bits used *) 
+      * simpl. autorewrite with eval_db; try lia.
+      * simpl. simpl in IHn0. simpl in H2.  assert (n0 > 0 -> S n0 > 0)%nat by lia.
+        rewrite IHn0. reflexivity.                    
+      try lia.
+      try lia.
+    + destruct (n mod 2 =? 1).
+      2:{unfold interpret_nexp_at. unfold interpret_nexp_at in IHn0. simpl in H1. rewrite IHn0. }
+Abort.
+*)
+(** Examples **)
+
+
+Infix "⊻" := b_xor (at level 40).
+Infix "∧" := b_and (at level 40).
+
+Local Close Scope R_scope.
+
+Set Printing Depth 100.
+
+(* Basic examples of compilation of plus and multiply without eval*)
+Definition simple_add : nexp := (n_plus (n_var_reg 0) (n_var_reg 1)).
+Redirect "out2" Eval compute in (n_compile simple_add 4).
+
+Definition num_nexp : nexp := (n_mult (n_plus (n_var_reg 0) (n_var_reg 1)) (n_var_reg 2)).
+Redirect "out2" Eval compute in (n_compile num_nexp 4).
+Eval cbv in (n_compile num_nexp 4).
+
+Definition multrec_nexp : nexp := (n_mult (n_plus (n_var_reg 0) (n_var_reg 1)) (n_var_reg 2)).
+Redirect "out2" Eval compute in (n_compile multrec_nexp 4).
+Eval cbv in (n_compile multrec_nexp 4).
+
+(* Incorporating evaluation *)
+Definition f_in2 : nat -> bool :=
+  fun n => (match n with
+            |0 => false
+            |S 0  => false
+            |S (S 0) => true
+            |S (S (S 0)) => true
+
+                    
+            |4 => false
+            |5 => false
+            |6 => true
+            |7 => true
+            |_ => false end).
+Eval compute in funbool_to_list 12 f_in2.
+Definition add_nexp : nexp := (n_plus (n_var_reg 1) (n_var_reg 0)).
+Definition add_nexp_compiled := (n_compile add_nexp 4).
+Eval compute in funbool_to_list 12 (bcexec add_nexp_compiled f_in2).
+Definition n_var_compiled : bccom := n_compile (n_var_reg 1 ) 4.
+Eval compute in funbool_to_list 12 (bcexec n_var_compiled f_in2).
+Eval compute in funbool_to_nat 4 (bcexec n_var_compiled f_in2).
+(*  n_compile_var   (i_in i_out i_anc n sz_reg: nat) : bccom   *)
+
+
+
+Definition simple_mult : nexp := (n_mult (n_var_reg 0) (n_var_reg 1)).
+Eval compute in interpret_nexp (n_var_reg 0) f_in2 4.
+Eval compute in interpret_nexp simple_mult f_in2 4.
+Definition mult_nexp_compiled := (n_compile simple_mult 4).
+Definition mult_nexp_interpreted := (bcexec mult_nexp_compiled f_in2).
+Eval compute in funbool_to_nat 4 (shift_vec_l mult_nexp_interpreted 8).
+Eval compute in funbool_to_nat 4 (nat_to_funbool 4 3).
+
+(** Testing more generally with QuickChick **)
+
+(*I want to, for now, use a list of nats to represent number stored in each register *)
+Fixpoint listnat_to_binlist (size : nat) (lst : list nat ) : list bool :=
+  match lst with
+
+  |nil => []
+  |h::t => (listnat_to_binlist size t)++(nat_to_binlist size h)
+  end. 
+
+Definition listnat_to_funbool (size : nat) (lst : list nat) : nat -> bool :=
+  let bl := (listnat_to_binlist size lst) in
+  list_to_funbool (List.length bl) (bl).
+
+(* making sure that the listnat can fit within the desired expression and reg size *)
+
+Fixpoint max_allowed_input_aux (size : nat) (ops : nexp) : nat :=
+  match ops with
+  |n_plus n1 n2 => min (max_allowed_input_aux (size - 1) n1) (max_allowed_input_aux (size - 1) n2)
+  |n_mult n1 n2 => min (max_allowed_input_aux (size / 2) n1) (max_allowed_input_aux (size /2) n2)
+  |_ => size
+  end.
+
+(*Note that this is too strict, there could be variations of numbers which would fit within
+the registers but aren't allowed. This will just be used for generators.  *)  
+Fixpoint max_allowed_input (size : nat) (ops : nexp) : nat :=
+   Nat.pow 2 (max_allowed_input_aux size ops) - 1.
+
+Eval compute in max_allowed_input 4 (n_mult (n_var_reg 0) (n_var_reg 1)).
+
+(*I'll now do tests on simple_add which is a circuit which just adds two numbers *)
+
+(*This generages lists of 2 nats, which we just need to transform into funbools. *)
+Sample (vectorOf 2 (choose (0, (max_allowed_input 4 simple_add) ))).
+
+
+Definition compile_matches (size : nat) (inputs : list nat) (e : nexp) :=
+  let f := listnat_to_funbool size inputs in
+  ((funbool_to_nat size (shift_vec_l (bcexec (n_compile e size) f) (size * (List.length inputs))))
+  = interpret_nexp e f size) ?.
+(*
+ QuickChick
+  (forAll
+     (vectorOf 2 (choose (0, (max_allowed_input 4 simple_add) )))
+     (fun i => compile_matches 4 i simple_add) 
+    ).
+Passes all tests.
+Note that if we had changed max_allowed_input to use +1 rather than -1, it would fail
+. One example being 9 + 7 which is 16, not expressible with 4 qubits*)
+(*
+QuickChick
+  (forAll
+     (choose (2, 10))
+     (fun size => (forAll (vectorOf 2 (choose (0, (max_allowed_input size simple_add) )))
+     (fun i =>
+        compile_matches size i simple_add)) 
+    )).
+It passes for a variety of register sizes.*)
+
+(*
+ QuickChick
+  (forAll
+     (vectorOf 2 (choose (0, (max_allowed_input 4 simple_mult) )))
+     (fun i => compile_matches 4 i simple_mult) 
+    ).
+I'm not going to vary the length of this much just because it takes an amount of time to compile
+circuits with large register sizes. 
+*)
+
+
+(** Now for the much harder (and longer to compute part) of generating nexps *)
+(* We want to generate expressions (and corresponding inputs) with the following characteristics:
+1) We need input to fit within input list
+2) The expression shouldn't be very deep (maybe 3 or 4 size max)
+3) The expression should be well typed 
+
+I suppose first we should generate random inputs, then random expressions from that?  
+
+*)
+Derive Show for nexp.
+
+Fixpoint gen_nexp_reg ( num_inputs : nat) : G (nexp) :=
+   bind (choose (0, num_inputs)) (fun x =>
+         ret (n_var_reg x)) .
+Sample (gen_nexp_reg 4).
+
+(* Need to change notation because bccom uses semicolons and I can't seem to close that scope*)
+Notation " 'freq' [ x ;;; y ] " := (freq_ (snd x) (cons x (cons y nil))) .
+Notation " 'freq' [ x ;;; y ;;; .. ;;; z ] " := (freq_ (snd x) (cons x (cons y .. (cons z nil) ..))).
+
+(*I am making n_plus twice as common as the two other possibilities because I don't want computation times to become too large *)
+Fixpoint gen_nexp_sized (sz num_inputs: nat) : G (nexp) :=
+  match sz with
+  | 0 => gen_nexp_reg num_inputs
+  | S sz' =>
+    freq[(1, (gen_nexp_reg num_inputs) ) ;;;
+         (2, (liftM2 n_plus (gen_nexp_sized sz' num_inputs) (gen_nexp_sized sz' num_inputs) )) ;;;
+         (1, (liftM2 n_mult (gen_nexp_sized sz' num_inputs) (gen_nexp_sized sz' num_inputs) ))
+        ]
+  end.
+
+Sample (gen_nexp_sized 2 4).
+
+Fixpoint num_in_regs (n : nexp):=
+  match n with
+  |n_plus n1 n2 => max (num_in_regs n1) (num_in_regs n2)
+  |n_mult n1 n2 => max (num_in_regs n1) (num_in_regs n2)
+  |n_var_reg r => r
+  |_ => 0
+  end.
+  
+
+(* using size of 4 and also 4 inputs just because it's small enough but not too small *)
+
+    
+
+Definition test_mult_plus_4 :=
+  forAll
+      (gen_nexp_sized 3 4)
+      (fun exp => let num_ins := ((num_in_regs exp)%nat + 1)%nat in
+                 forAll( (vectorOf num_ins (choose (0, (max_allowed_input 4 exp)))))
+                          (fun i => compile_matches 4 i exp)).
+ (*QuickChick
+   test_mult_plus_4.
+This works for gen_nexp_sized 3 4! Now to test with more range *)
+
+Definition test_mult_plus :=
+  forAll
+    (choose(1,6))
+    (fun reg_size => forAll
+      (gen_nexp_sized 3 reg_size)
+      (fun exp => let num_ins := ((num_in_regs exp)%nat + 1)%nat in
+                 forAll( (vectorOf num_ins (choose (0, (max_allowed_input reg_size exp)))))
+                          (fun i => compile_matches reg_size i exp))).
+
+(*QuickChick test_mult_plus.
+test_mult_plus is a more generic test than any we have done before. I am reluctant to test register sizes larger than six because of the amount of time it would take to run all the tests. 
+ 
+It is  also for this reason that I hesitate to increase the fuel parameter of gen_nexp_sized beyond 3
+*)
